<?xml version="1.0"?>
<rdf:RDF xmlns="http://purl.obolibrary.org/obo/tso/ENVO_import.owl#"
     xml:base="http://purl.obolibrary.org/obo/tso/ENVO_import.owl"
     xmlns:rdf="http://www.w3.org/1999/02/22-rdf-syntax-ns#"
     xmlns:owl="http://www.w3.org/2002/07/owl#"
     xmlns:oboInOwl="http://www.geneontology.org/formats/oboInOwl#"
     xmlns:xsd="http://www.w3.org/2001/XMLSchema#"
     xmlns:rdfs="http://www.w3.org/2000/01/rdf-schema#"
     xmlns:obo="http://purl.obolibrary.org/obo/"
     xmlns:dc="http://purl.org/dc/elements/1.1/">
    <owl:Ontology rdf:about="http://purl.obolibrary.org/obo/tso/ENVO_import.owl"/>
    


    <!-- 
    ///////////////////////////////////////////////////////////////////////////////////////
    //
    // Annotation properties
    //
    ///////////////////////////////////////////////////////////////////////////////////////
     -->

    <owl:AnnotationProperty rdf:about="http://purl.obolibrary.org/obo/IAO_0000117">
        <rdfs:label>term editor</rdfs:label>
    </owl:AnnotationProperty>
    <owl:AnnotationProperty rdf:about="http://purl.obolibrary.org/obo/IAO_0000119">
        <rdfs:label>definition source</rdfs:label>
    </owl:AnnotationProperty>
    <owl:AnnotationProperty rdf:about="http://purl.obolibrary.org/obo/IAO_0000116">
        <rdfs:label>editor note</rdfs:label>
    </owl:AnnotationProperty>
    <owl:AnnotationProperty rdf:about="http://purl.obolibrary.org/obo/IAO_0000412">
        <rdfs:label xml:lang="en">imported from</rdfs:label>
    </owl:AnnotationProperty>
    <owl:AnnotationProperty rdf:about="http://purl.obolibrary.org/obo/IAO_0000115">
        <rdfs:label rdf:datatype="http://www.w3.org/2001/XMLSchema#string">definition</rdfs:label>
    </owl:AnnotationProperty>
    <owl:AnnotationProperty rdf:about="http://www.geneontology.org/formats/oboInOwl#hasDbXref">
        <rdfs:label rdf:datatype="http://www.w3.org/2001/XMLSchema#string">database_cross_reference</rdfs:label>
    </owl:AnnotationProperty>
    <owl:AnnotationProperty rdf:about="http://www.geneontology.org/formats/oboInOwl#hasRelatedSynonym">
        <rdfs:label rdf:datatype="http://www.w3.org/2001/XMLSchema#string">has_related_synonym</rdfs:label>
    </owl:AnnotationProperty>
    <owl:AnnotationProperty rdf:about="http://www.geneontology.org/formats/oboInOwl#id"/>
    <owl:AnnotationProperty rdf:about="http://www.w3.org/2000/01/rdf-schema#comment"/>
    <owl:AnnotationProperty rdf:about="http://www.geneontology.org/formats/oboInOwl#hasBroadSynonym">
        <rdfs:label rdf:datatype="http://www.w3.org/2001/XMLSchema#string">has_broad_synonym</rdfs:label>
    </owl:AnnotationProperty>
    <owl:AnnotationProperty rdf:about="http://www.geneontology.org/formats/oboInOwl#hasOBONamespace">
        <rdfs:label rdf:datatype="http://www.w3.org/2001/XMLSchema#string">has_obo_namespace</rdfs:label>
    </owl:AnnotationProperty>
    <owl:AnnotationProperty rdf:about="http://www.geneontology.org/formats/oboInOwl#hasExactSynonym">
        <rdfs:label rdf:datatype="http://www.w3.org/2001/XMLSchema#string">has_exact_synonym</rdfs:label>
    </owl:AnnotationProperty>
    <owl:AnnotationProperty rdf:about="http://www.w3.org/2000/01/rdf-schema#label"/>
    <owl:AnnotationProperty rdf:about="http://www.geneontology.org/formats/oboInOwl#inSubset">
        <rdfs:label rdf:datatype="http://www.w3.org/2001/XMLSchema#string">in_subset</rdfs:label>
    </owl:AnnotationProperty>
    <owl:AnnotationProperty rdf:about="http://purl.org/dc/elements/1.1/creator"/>
    


    <!-- 
    ///////////////////////////////////////////////////////////////////////////////////////
    //
    // Datatypes
    //
    ///////////////////////////////////////////////////////////////////////////////////////
     -->

    


    <!-- 
    ///////////////////////////////////////////////////////////////////////////////////////
    //
    // Classes
    //
    ///////////////////////////////////////////////////////////////////////////////////////
     -->

    


    <!-- http://purl.obolibrary.org/obo/BFO_0000001 -->

    <owl:Class rdf:about="http://purl.obolibrary.org/obo/BFO_0000001">
        <rdfs:label xml:lang="en">entity</rdfs:label>
        <obo:IAO_0000412 rdf:resource="http://purl.obolibrary.org/obo/envo.owl"/>
    </owl:Class>
    


    <!-- http://purl.obolibrary.org/obo/BFO_0000002 -->

    <owl:Class rdf:about="http://purl.obolibrary.org/obo/BFO_0000002">
        <rdfs:label xml:lang="en">continuant</rdfs:label>
        <rdfs:subClassOf rdf:resource="http://purl.obolibrary.org/obo/BFO_0000001"/>
        <obo:IAO_0000115 xml:lang="en">An entity that exists in full at any time in which it exists at all, persists through time while maintaining its identity and has no temporal parts.</obo:IAO_0000115>
        <obo:IAO_0000412 rdf:resource="http://purl.obolibrary.org/obo/envo.owl"/>
    </owl:Class>
    


    <!-- http://purl.obolibrary.org/obo/BFO_0000003 -->

    <owl:Class rdf:about="http://purl.obolibrary.org/obo/BFO_0000003">
        <rdfs:label xml:lang="en">occurrent</rdfs:label>
        <rdfs:subClassOf rdf:resource="http://purl.obolibrary.org/obo/BFO_0000001"/>
        <obo:IAO_0000115 xml:lang="en">An entity that has temporal parts and that happens, unfolds or develops through time.</obo:IAO_0000115>
        <obo:IAO_0000412 rdf:resource="http://purl.obolibrary.org/obo/envo.owl"/>
    </owl:Class>
    


    <!-- http://purl.obolibrary.org/obo/BFO_0000004 -->

    <owl:Class rdf:about="http://purl.obolibrary.org/obo/BFO_0000004">
        <rdfs:label xml:lang="en">independent continuant</rdfs:label>
        <rdfs:subClassOf rdf:resource="http://purl.obolibrary.org/obo/BFO_0000002"/>
        <obo:IAO_0000115 xml:lang="en">A continuant that is a bearer of quality and realizable entity entities, in which other entities inhere and which itself cannot inhere in anything.</obo:IAO_0000115>
        <obo:IAO_0000115 xml:lang="en">b is an independent continuant = Def. b is a continuant which is such that there is no c and no t such that b s-depends_on c at t. (axiom label in BFO2 Reference: [017-002])</obo:IAO_0000115>
        <obo:IAO_0000412 rdf:resource="http://purl.obolibrary.org/obo/envo.owl"/>
    </owl:Class>
    


    <!-- http://purl.obolibrary.org/obo/BFO_0000015 -->

    <owl:Class rdf:about="http://purl.obolibrary.org/obo/BFO_0000015">
        <rdfs:label xml:lang="en">process</rdfs:label>
        <rdfs:subClassOf rdf:resource="http://purl.obolibrary.org/obo/BFO_0000003"/>
        <obo:IAO_0000115 xml:lang="en">An occurrent that has temporal proper parts and for some time t, p s-depends_on some material entity at t.</obo:IAO_0000115>
        <obo:IAO_0000115 xml:lang="en">p is a process = Def. p is an occurrent that has temporal proper parts and for some time t, p s-depends_on some material entity at t. (axiom label in BFO2 Reference: [083-003])</obo:IAO_0000115>
        <obo:IAO_0000412 rdf:resource="http://purl.obolibrary.org/obo/envo.owl"/>
    </owl:Class>
    


    <!-- http://purl.obolibrary.org/obo/BFO_0000029 -->

    <owl:Class rdf:about="http://purl.obolibrary.org/obo/BFO_0000029">
        <rdfs:label xml:lang="en">site</rdfs:label>
        <rdfs:subClassOf rdf:resource="http://purl.obolibrary.org/obo/BFO_0000141"/>
        <obo:IAO_0000412 rdf:resource="http://purl.obolibrary.org/obo/envo.owl"/>
    </owl:Class>
    


    <!-- http://purl.obolibrary.org/obo/BFO_0000040 -->

    <owl:Class rdf:about="http://purl.obolibrary.org/obo/BFO_0000040">
        <rdfs:label xml:lang="en">material entity</rdfs:label>
        <rdfs:subClassOf rdf:resource="http://purl.obolibrary.org/obo/BFO_0000004"/>
        <obo:IAO_0000115 xml:lang="en">An independent continuant that is spatially extended whose identity is independent of that of other entities and can be maintained through time.</obo:IAO_0000115>
        <obo:IAO_0000412 rdf:resource="http://purl.obolibrary.org/obo/envo.owl"/>
    </owl:Class>
    


    <!-- http://purl.obolibrary.org/obo/BFO_0000141 -->

    <owl:Class rdf:about="http://purl.obolibrary.org/obo/BFO_0000141">
        <rdfs:label xml:lang="en">immaterial entity</rdfs:label>
        <rdfs:subClassOf rdf:resource="http://purl.obolibrary.org/obo/BFO_0000004"/>
        <obo:IAO_0000412 rdf:resource="http://purl.obolibrary.org/obo/envo.owl"/>
    </owl:Class>
    


    <!-- http://purl.obolibrary.org/obo/ENVO_00000062 -->

    <owl:Class rdf:about="http://purl.obolibrary.org/obo/ENVO_00000062">
        <rdfs:label rdf:datatype="http://www.w3.org/2001/XMLSchema#string">populated place</rdfs:label>
        <rdfs:subClassOf rdf:resource="http://purl.obolibrary.org/obo/ENVO_01000408"/>
        <oboInOwl:hasOBONamespace rdf:datatype="http://www.w3.org/2001/XMLSchema#string">ENVO</oboInOwl:hasOBONamespace>
        <oboInOwl:id rdf:datatype="http://www.w3.org/2001/XMLSchema#string">ENVO:00000062</oboInOwl:id>
        <oboInOwl:hasDbXref rdf:datatype="http://www.w3.org/2001/XMLSchema#string">FTT:1097</oboInOwl:hasDbXref>
        <oboInOwl:hasDbXref rdf:datatype="http://www.w3.org/2001/XMLSchema#string">FTT:33</oboInOwl:hasDbXref>
        <oboInOwl:hasDbXref rdf:datatype="http://www.w3.org/2001/XMLSchema#string">Geonames:P.PPL</oboInOwl:hasDbXref>
        <oboInOwl:hasDbXref rdf:datatype="http://www.w3.org/2001/XMLSchema#string">Geonames:P.PPLS</oboInOwl:hasDbXref>
        <obo:IAO_0000115 rdf:datatype="http://www.w3.org/2001/XMLSchema#string">Place or area with clustered or scattered buildings and a permanent human population.</obo:IAO_0000115>
        <oboInOwl:hasDbXref rdf:datatype="http://www.w3.org/2001/XMLSchema#string">TGN:22201</oboInOwl:hasDbXref>
        <oboInOwl:hasDbXref rdf:datatype="http://www.w3.org/2001/XMLSchema#string">TGN:83002</oboInOwl:hasDbXref>
        <oboInOwl:hasDbXref rdf:datatype="http://www.w3.org/2001/XMLSchema#string">https://en.wikipedia.org/wiki/Populated_place</oboInOwl:hasDbXref>
        <oboInOwl:hasExactSynonym rdf:datatype="http://www.w3.org/2001/XMLSchema#string">inhabited place</oboInOwl:hasExactSynonym>
        <oboInOwl:hasRelatedSynonym rdf:datatype="http://www.w3.org/2001/XMLSchema#string">inhabited region</oboInOwl:hasRelatedSynonym>
        <oboInOwl:hasBroadSynonym rdf:datatype="http://www.w3.org/2001/XMLSchema#string">place</oboInOwl:hasBroadSynonym>
        <oboInOwl:hasRelatedSynonym rdf:datatype="http://www.w3.org/2001/XMLSchema#string">populated locality</oboInOwl:hasRelatedSynonym>
        <oboInOwl:hasExactSynonym rdf:datatype="http://www.w3.org/2001/XMLSchema#string">populated place</oboInOwl:hasExactSynonym>
        <oboInOwl:hasExactSynonym rdf:datatype="http://www.w3.org/2001/XMLSchema#string">populated places</oboInOwl:hasExactSynonym>
        <oboInOwl:hasExactSynonym rdf:datatype="http://www.w3.org/2001/XMLSchema#string">settlement</oboInOwl:hasExactSynonym>
        <obo:IAO_0000412 rdf:resource="http://purl.obolibrary.org/obo/envo.owl"/>
    </owl:Class>
    


    <!-- http://purl.obolibrary.org/obo/ENVO_00000856 -->

    <owl:Class rdf:about="http://purl.obolibrary.org/obo/ENVO_00000856">
        <rdfs:label rdf:datatype="http://www.w3.org/2001/XMLSchema#string">city</rdfs:label>
        <rdfs:subClassOf rdf:resource="http://purl.obolibrary.org/obo/ENVO_01000658"/>
        <oboInOwl:hasOBONamespace rdf:datatype="http://www.w3.org/2001/XMLSchema#string">ENVO</oboInOwl:hasOBONamespace>
        <oboInOwl:id rdf:datatype="http://www.w3.org/2001/XMLSchema#string">ENVO:00000856</oboInOwl:id>
        <oboInOwl:hasDbXref rdf:datatype="http://www.w3.org/2001/XMLSchema#string">EcoLexicon:city</oboInOwl:hasDbXref>
        <oboInOwl:hasDbXref rdf:datatype="http://www.w3.org/2001/XMLSchema#string">FTT:430</oboInOwl:hasDbXref>
        <oboInOwl:hasDbXref rdf:datatype="http://www.w3.org/2001/XMLSchema#string">FTT:483</oboInOwl:hasDbXref>
        <oboInOwl:hasDbXref rdf:datatype="http://www.w3.org/2001/XMLSchema#string">FTT:484</oboInOwl:hasDbXref>
        <oboInOwl:hasDbXref rdf:datatype="http://www.w3.org/2001/XMLSchema#string">FTT:485</oboInOwl:hasDbXref>
        <obo:IAO_0000115 rdf:datatype="http://www.w3.org/2001/XMLSchema#string">Incorporated populated place.</obo:IAO_0000115>
        <oboInOwl:hasDbXref rdf:datatype="http://www.w3.org/2001/XMLSchema#string">SWEETRealm:City</oboInOwl:hasDbXref>
        <oboInOwl:hasDbXref rdf:datatype="http://www.w3.org/2001/XMLSchema#string">TGN:83020</oboInOwl:hasDbXref>
        <oboInOwl:hasDbXref rdf:datatype="http://www.w3.org/2001/XMLSchema#string">TGN:83040</oboInOwl:hasDbXref>
        <oboInOwl:hasDbXref rdf:datatype="http://www.w3.org/2001/XMLSchema#string">TGN:83043</oboInOwl:hasDbXref>
        <oboInOwl:hasDbXref rdf:datatype="http://www.w3.org/2001/XMLSchema#string">https://en.wikipedia.org/wiki/City</oboInOwl:hasDbXref>
        <oboInOwl:hasBroadSynonym rdf:datatype="http://www.w3.org/2001/XMLSchema#string">urban area</oboInOwl:hasBroadSynonym>
        <obo:IAO_0000412 rdf:resource="http://purl.obolibrary.org/obo/envo.owl"/>
    </owl:Class>
    


    <!-- http://purl.obolibrary.org/obo/ENVO_01000408 -->

    <owl:Class rdf:about="http://purl.obolibrary.org/obo/ENVO_01000408">
        <rdfs:label>environmental zone</rdfs:label>
        <rdfs:subClassOf rdf:resource="http://purl.obolibrary.org/obo/BFO_0000029"/>
        <obo:IAO_0000115 rdf:datatype="http://www.w3.org/2001/XMLSchema#string">A site which has its extent determined by the presence or influence of one or more components of an environmental system or the processes occurring therein.</obo:IAO_0000115>
        <rdfs:comment rdf:datatype="http://www.w3.org/2001/XMLSchema#string">Formerly, this class was an experimental class and a subclass of &quot;environmental feature&quot;. It is now aligned to BFO. The class was not obsoleted as the core semantics maintained their stability through its transition.</rdfs:comment>
        <oboInOwl:hasRelatedSynonym rdf:datatype="http://www.w3.org/2001/XMLSchema#string">environmental area</oboInOwl:hasRelatedSynonym>
        <oboInOwl:inSubset>envoPolar</oboInOwl:inSubset>
        <obo:IAO_0000412 rdf:resource="http://purl.obolibrary.org/obo/envo.owl"/>
    </owl:Class>
    


    <!-- http://purl.obolibrary.org/obo/ENVO_01000658 -->

    <owl:Class rdf:about="http://purl.obolibrary.org/obo/ENVO_01000658">
        <rdfs:label xml:lang="en">dense settlement</rdfs:label>
        <rdfs:subClassOf rdf:resource="http://purl.obolibrary.org/obo/ENVO_00000062"/>
        <obo:IAO_0000115>A settlement with a high density of buildings and inhabitants.</obo:IAO_0000115>
        <rdfs:comment>The thresholds for what makes a settlment &quot;dense&quot; can be determined as needed. If there is a specific threshold that should be added to ENVO, please make a new class request.</rdfs:comment>
        <obo:IAO_0000116>See also: http://www.ecotope.org/anthromes/v1/guide/urban/12_dense_settlements/default.aspx</obo:IAO_0000116>
        <obo:IAO_0000412 rdf:resource="http://purl.obolibrary.org/obo/envo.owl"/>
    </owl:Class>
    


    <!-- http://purl.obolibrary.org/obo/ENVO_01000772 -->

    <owl:Class rdf:about="http://purl.obolibrary.org/obo/ENVO_01000772">
        <rdfs:label xml:lang="en">rural area</rdfs:label>
        <rdfs:subClassOf rdf:resource="http://purl.obolibrary.org/obo/ENVO_01001200"/>
        <rdfs:comment>A class created fro SDGIO. The definition of rural is highly varied, dealing with areas, settlements, and populations interchangeably. The &#39;rural&#39; classes in ENVO aim to clarify these differing definitions. See issue #272.</rdfs:comment>
        <obo:IAO_0000115>An area which is outside of a town, city, or urban area. Rural areas are primarily used for agriculture or pastoralism and may contain rural settlements.</obo:IAO_0000115>
        <obo:IAO_0000412 rdf:resource="http://purl.obolibrary.org/obo/envo.owl"/>
    </owl:Class>
    


    <!-- http://purl.obolibrary.org/obo/ENVO_01001199 -->

    <owl:Class rdf:about="http://purl.obolibrary.org/obo/ENVO_01001199">
        <rdfs:label xml:lang="en">terrestrial environmental zone</rdfs:label>
        <rdfs:subClassOf rdf:resource="http://purl.obolibrary.org/obo/ENVO_01000408"/>
        <obo:IAO_0000115>An environmental zone which is bounded by material parts of a land mass or the atmosphere or space adjacent to it.</obo:IAO_0000115>
        <obo:IAO_0000412 rdf:resource="http://purl.obolibrary.org/obo/envo.owl"/>
    </owl:Class>
    


    <!-- http://purl.obolibrary.org/obo/ENVO_01001200 -->

    <owl:Class rdf:about="http://purl.obolibrary.org/obo/ENVO_01001200">
        <rdfs:label xml:lang="en">anthropised terrestrial environmental zone</rdfs:label>
        <rdfs:subClassOf rdf:resource="http://purl.obolibrary.org/obo/ENVO_01001199"/>
        <obo:IAO_0000115>A terrestrial zone which is bounded by constructed, manufactured, or other anthropogenic material entities.</obo:IAO_0000115>
        <obo:IAO_0000412 rdf:resource="http://purl.obolibrary.org/obo/envo.owl"/>
    </owl:Class>
    


    <!-- http://purl.obolibrary.org/obo/ENVO_02000125 -->

    <owl:Class rdf:about="http://purl.obolibrary.org/obo/ENVO_02000125">
        <rdfs:label>transportation</rdfs:label>
        <rdfs:subClassOf rdf:resource="http://purl.obolibrary.org/obo/ENVO_03000010"/>
        <dc:creator rdf:datatype="http://www.w3.org/2001/XMLSchema#string">cjm</dc:creator>
        <obo:IAO_0000115>A planned process that is the movement of people, animals and goods from one location to another.</obo:IAO_0000115>
        <obo:IAO_0000412 rdf:resource="http://purl.obolibrary.org/obo/envo.owl"/>
    </owl:Class>
    


    <!-- http://purl.obolibrary.org/obo/ENVO_02500000 -->

    <owl:Class rdf:about="http://purl.obolibrary.org/obo/ENVO_02500000">
        <rdfs:label xml:lang="en">environmental system process</rdfs:label>
        <rdfs:subClassOf rdf:resource="http://purl.obolibrary.org/obo/BFO_0000015"/>
        <rdfs:comment>This is a convenience class for organisation and should not be used for annotation.</rdfs:comment>
        <obo:IAO_0000115>A process in which includes the components of an environmental system as participants.</obo:IAO_0000115>
        <obo:IAO_0000412 rdf:resource="http://purl.obolibrary.org/obo/envo.owl"/>
    </owl:Class>
    


    <!-- http://purl.obolibrary.org/obo/ENVO_03000010 -->

    <owl:Class rdf:about="http://purl.obolibrary.org/obo/ENVO_03000010">
        <rdfs:label xml:lang="en">material transport process</rdfs:label>
        <rdfs:subClassOf rdf:resource="http://purl.obolibrary.org/obo/ENVO_02500000"/>
        <obo:IAO_0000117>http://orcid.org/0000-0002-4366-3088</obo:IAO_0000117>
        <obo:IAO_0000115>A process during which material is displaced from its original location and transported either to a new location or back to the original location.</obo:IAO_0000115>
        <obo:IAO_0000117>http://orcid.org/0000-0002-3410-4655</obo:IAO_0000117>
        <oboInOwl:inSubset>envoPolar</oboInOwl:inSubset>
        <rdfs:comment>Experimental class for structural purposes not recommended for annotation.</rdfs:comment>
        <obo:IAO_0000412 rdf:resource="http://purl.obolibrary.org/obo/envo.owl"/>
    </owl:Class>
    


    <!-- http://purl.obolibrary.org/obo/RO_0002577 -->

    <owl:Class rdf:about="http://purl.obolibrary.org/obo/RO_0002577">
        <rdfs:label>system</rdfs:label>
        <rdfs:subClassOf rdf:resource="http://purl.obolibrary.org/obo/BFO_0000040"/>
        <obo:IAO_0000116>May be replaced by a BFO class, as discussed in http://www.jbiomedsem.com/content/4/1/43</obo:IAO_0000116>
        <obo:IAO_0000117>Chris Mungall</obo:IAO_0000117>
        <obo:IAO_0000115>A material entity consisting of multiple components that are causally integrated.</obo:IAO_0000115>
        <obo:IAO_0000119>http://www.jbiomedsem.com/content/4/1/43</obo:IAO_0000119>
        <obo:IAO_0000412 rdf:resource="http://purl.obolibrary.org/obo/envo.owl"/>
    </owl:Class>
</rdf:RDF>



<!-- Generated by the OWL API (version 1.3.5.1016) http://owlapi.sourceforge.net -->

